Balloc.v: lots of progress (moving to RecArray)
I moved virtually all of Inode.v to RecArray.v since it was all useful
for Balloc.v.

src/Balloc.v
@@ -14,6 +14,10 @@ Require Import Nomega.
 Require Import Idempotent.
 Require Import Psatz.
 Require Import AddrMap.
+Require Import Rec.
+Require Import RecArray.
+Require Import NArith.
+
 
 Set Implicit Arguments.
 
@@ -21,30 +25,55 @@ Set Implicit Arguments.
 (* Block allocator *)
 
 Record xparams := {
-    BmapStart : addr;
+  BmapStart : addr;
   BmapNBlocks : addr
 }.
 
 Module BALLOC.
+
+  Definition itemtype := Rec.WordF 1.
+  Definition items_per_valu : addr := natToWord addrlen valulen.
+  Theorem items_per_valu_not_0 : items_per_valu <> $0.
+    Require Import WordAuto.
+    unfold items_per_valu. rewrite valulen_is. apply word_neq. compute. intro H. simpl in H. discriminate.
+  Qed.
+
+  Theorem blocksz : valulen = Rec.len (RecArray.blocktype itemtype items_per_valu).
+    unfold blocktype, items_per_valu.
+    rewrite wordToNat_natToWord_idempotent.
+    simpl. ring.
+    rewrite valulen_is. compute. auto.
+  Qed.
+
+  Definition rep_block := RecArray.rep_block blocksz.
+  Definition valu_to_block := RecArray.valu_to_block itemtype items_per_valu blocksz.
+  Definition rep_valu_id := RecArray.rep_valu_id blocksz.
+
+
   Inductive alloc_state :=
   | Avail
   | InUse.
 
-  Definition alloc_state_to_valu a pos : valu :=
+  Definition alloc_state_dec : forall (a b : alloc_state), {a = b} + {a <> b}.
+    destruct a; destruct b; try (left; constructor); right; discriminate.
+  Qed.
+
+  Definition alloc_state_to_bit a : word 1 :=
     match a with
     | Avail => $0
-    | InUse => wbit _ ($ pos : addr)
+    | InUse => $1
     end.
 
-  Definition blockbits (bmap : addr -> alloc_state) offset :=
-    fold_right (@wor _) $0
-               (map (fun i => alloc_state_to_valu (bmap $ (offset + i)) i)
-                    (seq 0 valulen)).
+  Definition bit_to_alloc_state (b : word 1) : alloc_state :=
+    match b with
+    | WS false W0 => Avail
+    | _ => InUse
+    end.
 
-  Definition rep' xp (bmap : addr -> alloc_state) :=
-    array (BmapStart xp)
-          (map (fun nblock => blockbits bmap (nblock * valulen))
-               (seq 0 (wordToNat (BmapNBlocks xp)))) $1.
+  Lemma bit_alloc_state_id : forall a, bit_to_alloc_state (alloc_state_to_bit a) = a.
+    destruct a; auto.
+  Qed.
+  Hint Rewrite bit_alloc_state_id.
 
   Theorem selN_list_eq' : forall A len (vs vs' : list A) default,
     length vs = len
@@ -78,193 +107,45 @@ Module BALLOC.
     induction vs; destruct n'; destruct n; simpl; intuition; try omega.
   Qed.
 
-  Hint Rewrite length_updN.
-  Hint Rewrite map_length.
-  Hint Rewrite seq_length.
+  Definition bmap_bits xp (bmap : addr -> alloc_state) :=
+     map (fun i => alloc_state_to_bit (bmap $ (i)))
+          (seq 0 (wordToNat (BmapNBlocks xp) * valulen)).
 
-  Theorem blockbits_bupd_other : forall bmap bn x i bnblock,
-    (bnblock ^* $ valulen <= bn)%word
-    -> (bn < bnblock ^* $ valulen ^+ $ valulen)%word
-    -> i <> wordToNat bnblock
-    -> blockbits (fupd bmap bn x) (i * valulen) = blockbits bmap (i * valulen).
-  Proof.
-    unfold blockbits.
-    intros.
-    f_equal.
-    eapply selN_list_eq with (default:=$0); autorewrite with core; auto.
+  Definition xp_to_raxp xp :=
+    RecArray.Build_xparams (BmapStart xp) (BmapNBlocks xp).
 
-    intros.
-    repeat rewrite selN_map_seq; auto.
-    f_equal.
-    rewrite fupd_other; auto.
-    unfold not in *; intros; apply H1; clear H1; subst.
-    admit.
-  Qed.
-
-  Theorem valulen_bound : valulen <= wordToNat ($ valulen : addr).
-  Proof.
-    rewrite wordToNat_natToWord_idempotent'; auto.
-    rewrite valulen_is.
-    unfold addrlen.
-    unfold pow2; omega.
-  Qed.
-
-  Theorem wordToNat_wminus : forall sz (a b : word sz), (b <= a)%word
-    -> wordToNat (a ^- b) = wordToNat a - wordToNat b.
-  Proof.
-    admit.
-  Qed.
-
-  Theorem blockbits_bupd_same_avail': forall vlen start bmap bn bnblock,
-    start + vlen = valulen
-    -> (bnblock ^* $ valulen <= bn)%word
-    -> (bn < bnblock ^* $ valulen ^+ $ valulen)%word
-    -> fold_right (wor (sz:=valulen)) $ (0)
-         (map (fun i : nat => alloc_state_to_valu (bmap $ (wordToNat bnblock * valulen + i)) i)
-            (seq start vlen)) ^& wnot (wbit valulen (bn ^- bnblock ^* $ (valulen))) =
-       fold_right (wor (sz:=valulen)) $ (0)
-         (map
-            (fun i : nat =>
-             alloc_state_to_valu (fupd bmap bn Avail $ (wordToNat bnblock * valulen + i)) i)
-            (seq start vlen)).
-  Proof.
-    induction vlen; simpl; intros.
-    rewrite wand_kill; auto.
-    rewrite wand_or_distr; f_equal.
-    - destruct (weq bn $ (wordToNat bnblock * valulen + start)).
-      + subst. rewrite fupd_same; auto. simpl.
-        destruct (bmap $ (wordToNat bnblock * valulen + start)); simpl; try apply wand_kill.
-        replace ($ (wordToNat bnblock * valulen + start) ^- bnblock ^* $ valulen)
-          with ($ start : addr) by words.
-        rewrite wbit_and_not; auto.
-        clear H0 H1 IHvlen.
-        erewrite wordToNat_natToWord_bound; try omega.
-        eapply le_trans; [| apply valulen_bound ].
-        omega.
-      + rewrite fupd_other; auto.
-        destruct (bmap $ (wordToNat bnblock * valulen + start)); simpl; try apply wand_kill.
-        rewrite wbit_and_not_other; auto.
-        erewrite wordToNat_natToWord_bound; try omega.
-        eapply le_trans; [| apply valulen_bound ]; omega.
-
-        rewrite wordToNat_wminus; auto.
-        apply wlt_lt in H1.
-        admit.
-
-        unfold not in *; intros; apply n.
-        rewrite natToWord_plus.
-        rewrite H2.
-        words.
-    - apply IHvlen; auto; omega.
-  Qed.
-
-  Theorem blockbits_bupd_same_avail : forall bmap bn bnblock,
-    (bnblock ^* $ valulen <= bn)%word
-    -> (bn < bnblock ^* $ valulen ^+ $ valulen)%word
-    -> blockbits bmap (wordToNat bnblock * valulen)
-         ^& wnot (wbit valulen (bn ^- bnblock ^* $ (valulen))) =
-       blockbits (fupd bmap bn Avail) (wordToNat bnblock * valulen).
-  Proof.
-    intros.
-    unfold blockbits.
-    rewrite blockbits_bupd_same_avail'; auto.
-  Qed.
-
-  Theorem blockbits_bupd_same_inuse : forall bmap bn bnblock,
-    (bnblock ^* $ valulen <= bn)%word
-    -> (bn < bnblock ^* $ valulen ^+ $ valulen)%word
-    -> blockbits bmap (wordToNat bnblock * valulen)
-         ^| wbit valulen (bn ^- bnblock ^* $ valulen) =
-       blockbits (fupd bmap bn InUse) (wordToNat bnblock * valulen).
-  Proof.
-    intros.
-    unfold blockbits.
-    admit.
-  Qed.
-
-  Theorem upd_bupd_avail : forall bmap astart nblocks bn bnblock oldblocks,
-    (bn >= bnblock ^* $ valulen)%word
-    -> (bn < bnblock ^* $ valulen ^+ $ valulen)%word
-    -> (bnblock < nblocks)%word
-    -> oldblocks = (map (fun nblock => blockbits bmap (nblock * valulen))
-                        (seq 0 (wordToNat nblocks)))
-    -> array astart (upd oldblocks bnblock
-                         (sel oldblocks bnblock $0 ^&
-                          wnot (wbit valulen (bn ^- bnblock ^* $ valulen)))) =
-       array astart
-         (map (fun nblock => blockbits (fupd bmap bn Avail) (nblock * valulen))
-              (seq 0 (wordToNat nblocks))).
-  Proof.
-    intros.
-    f_equal.
-    unfold upd.
-    eapply selN_list_eq.
-    - subst; autorewrite with core. auto.
-    - unfold sel; intros.
-      apply wlt_lt in H1 as H1'.
-      destruct (eq_nat_dec (wordToNat bnblock) i); subst.
-      + rewrite selN_updN_eq; autorewrite with core; auto.
-        repeat rewrite selN_map_seq; auto.
-        erewrite blockbits_bupd_same_avail; eauto.
-      + autorewrite with core in *.
-        rewrite selN_updN_ne; autorewrite with core; auto.
-        erewrite blockbits_bupd_other; eauto.
-  Qed.
-
-  Theorem upd_bupd_inuse : forall bmap astart nblocks bnblock bnoff oldblocks,
-    (bnoff < $ valulen)%word
-    -> (bnblock < nblocks)%word
-    -> oldblocks = (map (fun nblock => blockbits bmap (nblock * valulen))
-                        (seq 0 (wordToNat nblocks)))
-    -> array astart (upd oldblocks bnblock
-                         (sel oldblocks bnblock $0 ^| wbit valulen bnoff)) =
-       array astart
-         (map (fun nblock => blockbits (fupd bmap (bnblock ^* $ valulen ^+ bnoff) InUse)
-                                       (nblock * valulen))
-              (seq 0 (wordToNat nblocks))).
-  Proof.
-    intros.
-    f_equal.
-    unfold upd.
-    eapply selN_list_eq.
-    - subst; autorewrite with core. auto.
-    - unfold sel; intros.
-      apply wlt_lt in H0 as H0'.
-      destruct (eq_nat_dec (wordToNat bnblock) i); subst.
-      + rewrite selN_updN_eq; autorewrite with core; auto.
-        repeat rewrite selN_map_seq; auto.
-        replace (bnoff) with ((bnblock ^* $ valulen ^+ bnoff) ^- bnblock ^* $ valulen) at 1 by ring.
-        erewrite blockbits_bupd_same_inuse; eauto.
-        admit.
-        admit.
-      + rewrite selN_updN_ne; autorewrite with core; auto.
-        autorewrite with core in *.
-        repeat rewrite selN_map_seq; auto.
-        erewrite blockbits_bupd_other; eauto.
-        admit.
-        admit.
-  Qed.
+  Definition rep' xp (bmap : addr -> alloc_state) :=
+    RecArray.array_item itemtype items_per_valu blocksz (xp_to_raxp xp)
+      (bmap_bits xp bmap).
 
   Definition free' T lxp xp bn rx : prog T :=
-    For i < (BmapNBlocks xp)
-      Ghost mbase m
-      Loopvar _ <- tt
-      Continuation lrx
-      Invariant
-        LOG.rep lxp (ActiveTxn mbase m) * [[ (i ^* $ valulen <= bn)%word ]]
-      OnCrash
-        LOG.log_intact lxp mbase
-      Begin
-        If (wlt_dec bn (i ^* $ valulen ^+ $ valulen)) {
-          b <- LOG.read_array lxp (BmapStart xp) i $1 ;
-          ok <- LOG.write_array lxp (BmapStart xp) i $1
-                (b ^& wnot (wbit _ (bn ^- (i ^* $ valulen)))) ;
-          rx ok
-        } else {
-          lrx tt
-        }
-    Rof ;;
-    rx false.
+    RecArray.put itemtype items_per_valu blocksz
+      lxp (xp_to_raxp xp) bn (alloc_state_to_bit Avail) rx.
+
+  (* The second hypothesis isn't actually necessary but makes things simpler *)
+  Lemma upd_bmap_bits : forall xp a bn b state,
+    b = alloc_state_to_bit state ->
+    wordToNat bn < wordToNat (BmapNBlocks xp) * valulen ->
+    upd (bmap_bits xp a) bn b = bmap_bits xp (fupd a bn state).
+  Proof.
+    intros. rewrite H. unfold bmap_bits, upd.
+    rewrite updN_map_seq.
+    apply list_selN_ext with (default := $ (0)).
+    repeat rewrite map_length; trivial.
+    intros pos Hl.
+    rewrite map_length in Hl. rewrite seq_length in Hl.
+    repeat rewrite selN_map with (default' := 0) by (rewrite seq_length; assumption).
+    Lemma selN_seq : forall a b c d, c < b -> selN (seq a b) c d = a + c.
+    Proof.
+      intros. rewrite nth_selN_eq. apply seq_nth; assumption.
+    Qed.
+    rewrite selN_seq by assumption. simpl.
+    destruct (Nat.eq_dec pos (wordToNat bn)).
+    rewrite e. rewrite natToWord_wordToNat. rewrite fupd_same; trivial.
+    rewrite fupd_other. trivial.
+    admit. (* XXX might need to worry about overflow here *)
+    assumption.
+  Qed.
 
   Theorem free'_ok : forall lxp xp bn,
     {< Fm mbase m bmap,
@@ -278,30 +159,25 @@ Module BALLOC.
     >} free' lxp xp bn.
   Proof.
     unfold free', rep', LOG.log_intact.
-    hoare.
+    intros. eapply pimpl_ok2. apply put_ok. (* XXX why doesn't eauto with prog work? *)
+    apply items_per_valu_not_0.
 
-    apply wlt_lt in H3.
-    ring_simplify ($ 0 ^* $ valulen : addr) in H3; simpl in H3; omega.
-
-    try rewrite map_length. try rewrite seq_length. apply wlt_lt. auto.
-    try rewrite map_length. try rewrite seq_length. apply wlt_lt. auto.
-
-    eapply pimpl_or_r; left.
     cancel.
-    admit.
-(*
-    erewrite upd_bupd_avail; eauto.
-*)
-
-    rewrite wmult_plus_distr in *.
-    rewrite wmult_unit in *.
-    auto.
+    step.
+    apply pimpl_or_r. left.
+    norm.
+    cancel.
+    repeat (split; [constructor |]).
+    pred_apply. cancel.
+    erewrite upd_bmap_bits; try trivial.
+    apply wlt_mult_inj in H4. rewrite wordToNat_natToWord_idempotent in H4. assumption.
+    simpl. rewrite valulen_is. compute. trivial.
   Qed.
 
   Hint Extern 1 ({{_}} progseq (free' _ _ _) _) => apply free'_ok : prog.
 
   Definition alloc' T lxp xp rx : prog T :=
-    For i < (BmapNBlocks xp)
+    For i < (BmapNBlocks xp ^* $ (valulen))
       Ghost mbase m
       Loopvar _ <- tt
       Continuation lrx
@@ -310,29 +186,20 @@ Module BALLOC.
       OnCrash
         LOG.log_intact lxp mbase
       Begin
-        blk <- LOG.read_array lxp (BmapStart xp) i $1;
-
-        For j < $ valulen
-          Ghost mbase' m'
-          Loopvar _ <- tt
-          Continuation lrx_inner
-          Invariant
-            LOG.rep lxp (ActiveTxn mbase' m')
-          OnCrash
-            LOG.log_intact lxp mbase'
-          Begin
-            If (weq (blk ^& wbit _ j) $0) {
-              ok <- LOG.write_array lxp (BmapStart xp) i $1 (blk ^| wbit _ j) ;
-              If (bool_dec ok true) {
-                rx (Some (i ^* $ valulen ^+ j))
-              } else {
-                rx None
-              }
-            } else {
-              lrx_inner tt
-            }
-          Rof;;
-        lrx tt
+        bit <- RecArray.get itemtype items_per_valu blocksz
+          lxp (xp_to_raxp xp) i;
+        let state := bit_to_alloc_state bit in
+        If (alloc_state_dec state Avail) {
+          ok <- RecArray.put itemtype items_per_valu blocksz
+            lxp (xp_to_raxp xp) i (alloc_state_to_bit InUse);
+          If (bool_dec ok true) {
+            rx (Some i)
+          } else {
+            rx None
+          }
+        } else {
+          lrx tt
+        }
       Rof;;
     rx None.
 
@@ -374,7 +241,7 @@ Module BALLOC.
     eapply sel_avail'; eauto.
     rewrite wplus_comm. rewrite wplus_unit. auto.
   Qed.
-*)
+
 
   Theorem sel_avail : forall bmap bnblock bnoff nblocks,
      sel (map (fun nblock => blockbits bmap (nblock * valulen))
@@ -388,10 +255,14 @@ Module BALLOC.
     rewrite selN_map_seq in H; auto.
     admit.
   Qed.
+*)
+
+  Hint Rewrite natToWord_wordToNat selN_map_seq.
 
   Theorem alloc'_ok: forall lxp xp,
     {< Fm mbase m bmap,
-    PRE    LOG.rep lxp (ActiveTxn mbase m) * [[ (Fm * rep' xp bmap)%pred m ]]
+    PRE    LOG.rep lxp (ActiveTxn mbase m) * [[ (Fm * rep' xp bmap)%pred m ]] *
+           [[ (wordToN (BmapNBlocks xp) * N.of_nat valulen < Npow2 addrlen)%N ]]
     POST:r [[ r = None ]] * LOG.rep lxp (ActiveTxn mbase m) \/
            exists bn m', [[ r = Some bn ]] * [[ bmap bn = Avail ]] *
            LOG.rep lxp (ActiveTxn mbase m') *
@@ -401,19 +272,25 @@ Module BALLOC.
   Proof.
     unfold alloc', rep', LOG.log_intact.
     hoare.
+    eapply pimpl_ok2. apply get_ok. (* XXX why doesn't eauto with prog work? *)
+    apply items_per_valu_not_0.
 
-    try rewrite map_length. try rewrite seq_length. apply wlt_lt. auto.
-    try rewrite map_length. try rewrite seq_length. apply wlt_lt. auto.
-
-    apply pimpl_or_r. right.
     cancel.
-
-(*     eapply sel_avail; try autorewrite_fast; eauto. *)
-    admit.
-    admit.
-(*
-    erewrite upd_bupd_inuse; eauto.
-*)
+    hoare.
+    eapply pimpl_ok2. apply put_ok.
+    apply items_per_valu_not_0.
+    cancel.
+    hoare.
+    apply pimpl_or_r. right.
+    (* XXX word automation *)
+    apply wlt_mult_inj in H3.
+    rewrite wordToNat_natToWord_idempotent in H3 by (simpl; rewrite valulen_is; compute; trivial).
+    cancel.
+    rewrite <- H10. unfold bmap_bits, sel.
+    autorewrite with core; auto.
+    erewrite upd_bmap_bits; trivial.
+    step.
+    step.
   Qed.
 
   Hint Extern 1 ({{_}} progseq (alloc' _) _) => apply alloc'_ok : prog.
